\section{Aufgabe 24}
\setcounter{section}{24}

Es seien $f : X \rightarrow Y$ eine Abbildung und $A, B \subset Y$. Zeigen Sie,
dass folgendes gilt:
\begin{equation*}
    \begin{gathered}
        f^{-1}(A \cap B) = f^{-1}(A) \cap f^{-1}(B)\text{,}\\
        f^{-1}(A \cup B) = f^{-1}(A) \cup f^{-1}(B)
    \end{gathered}
\end{equation*}

\begin{equation*}
    \begin{aligned}
        f^{-1}(A \cap B) &= \{x \in X : f(x) \in \{A \cap B\}\} = \\
                         &= \{x \in X : f(x) \in A \text{ und } f(x) \in B\} = \\
                         &= \{x \in X : f(x) \in A\} \cap \{x \in X : f(x) \in B\} = \\
                         &= f^{-1}(A) \cap f^{-1}(B) \quad \text{\underline{q.e.d.}}
    \end{aligned}
\end{equation*}

\begin{equation*}
    \begin{aligned}
        f^{-1}(A \cup B) &= \{x \in X : f(x) \in \{A \cup B\}\} = \\
                         &= \{x \in X : f(x) \in A \text{ oder } f(x) \in B\} = \\
                         &= \{x \in X : f(x) \in A\} \cup \{x \in X : f(x) \in B\} = \\
                         &= f^{-1}(A) \cup f^{-1}(B) \quad \text{\underline{q.e.d.}}
    \end{aligned}
\end{equation*}
