\section{Aufgabe 7}

\begin{align*}
    v + w           &= \sum_{j = 1}^n\alpha_j \cdot v_j + \sum_{j = 1}^n\beta_j \cdot v_j = \sum_{j = 1}^n\alpha_j \cdot v_j + \beta_j \cdot v_j = \sum_{j = 1}^n(\alpha_j + \beta_j) \cdot v_j = \\
                    &= \sum_{j = 1}^n\lambda_j \cdot v_j \ \ \ (\in \text{Span}(v_1, ..., v_m)) \ \ \ \square \\[10pt]
    \lambda \cdot v &= \lambda \cdot \sum_{j = 1}^n\alpha_j \cdot v_j = \sum_{j = 1}^n(\lambda \cdot \alpha_j) \cdot v_j \\
                    &= \sum_{j = 1}^n\lambda_j \cdot v_j \ \ \ (\in \text{Span}(v_1, ..., v_m)) \ \ \ \square
\end{align*}
