\section{Aufgabe 46}
\setcounter{section}{46}

Es sei $\Omega = \{0, 1\}^3$ mit $P(\{\omega\}) = \dfrac{1}{8}$ $(\omega \in \Omega)$ unser W-Raum. Dann gilt
\begin{equation*}
    \Omega = \{(0, 0, 0), (0, 0, 1), (0, 1, 0), (0, 1, 1), (1, 0, 0), (1, 0, 1), (1, 1, 0), (1, 1, 1)\}
\end{equation*}
Daraus ergibt sich das Folgende:
\begin{enumerate}[i)]
    \item $P(X = 4 | Y = f_1) = \dfrac{6}{8} = \dfrac{3}{4}$
    \item $P(X = 4 | Y = f_2) = \dfrac{2}{8} = \dfrac{1}{4}$
    \item $P(X = 4 | Y = f_3) = \dfrac{3}{8}$
\end{enumerate}
Gem"a{\ss} der Bayes-Formel (6.49 im Skript) gilt
\begin{equation*}
    P(Y = f_l | X = 4) = \dfrac{P(X = 4 | Y = f_l)P(Y = f_l)}{\sum_{j = 1}^nP(X = 4 | Y = f_j)P(Y = f_j)}
\end{equation*}
Daraus folgt
\begin{enumerate}[i)]
    \item $\begin{aligned}[t]
            P(Y = f_1 | X = 4) &= \dfrac{P(X = 4 | Y = f_1)P(Y = f_1)}{\sum_{j = 1}^3P(X = 4 | Y = f_j)P(Y = f_j)}  \\[5pt]
                               &= \dfrac{6/8 \cdot 1/3}{6/8 \cdot 1/3 + 2/8 \cdot 1/3 + 3/8 \cdot 1/3} = \dfrac{6}{11}
        \end{aligned}$ \\[5pt]
    \item $\begin{aligned}[t]
            P(Y = f_2 | X = 4) &= \dfrac{P(X = 4 | Y = f_2)P(Y = f_2)}{\sum_{j = 1}^3P(X = 4 | Y = f_j)P(Y = f_j)}  \\[5pt]
                               &= \dfrac{2/8 \cdot 1/3}{6/8 \cdot 1/3 + 2/8 \cdot 1/3 + 3/8 \cdot 1/3} = \dfrac{2}{11}
        \end{aligned}$ \\[5pt]
    \item $\begin{aligned}[t]
            P(Y = f_3 | X = 4) &= \dfrac{P(X = 4 | Y = f_3)P(Y = f_3)}{\sum_{j = 1}^3P(X = 4 | Y = f_j)P(Y = f_j)}  \\[5pt]
                               &= \dfrac{3/8 \cdot 1/3}{6/8 \cdot 1/3 + 2/8 \cdot 1/3 + 3/8 \cdot 1/3} = \dfrac{3}{11}
        \end{aligned}$
\end{enumerate}
