\section{Aufgabe 26}
\setcounter{section}{26}

Beweisen Sie die Aussage $P(A \cup B) = P(A) + P(B) - P(A \cap B)$.
\begin{equation*}
    \begin{aligned}
        A \cup B &= (A \setminus B) \cup (B \setminus A) \cup (A \cap B) \\[5pt]
        P(A \setminus B) &= P(A) - P(A \cap B) \\[5pt]
        P(B \setminus A) &= P(B) - P(A \cap B) \\[5pt]
        P(A \cup B) &= P(A \setminus B) + P(B \setminus A) + P(A \cap B) = \\[5pt]
                    &= (P(A) - P(A \cap B)) + (P(B) - P(A \cap B)) + P(A \cap B) = \\[5pt]
                    &= P(A) + P(B) + P(A \cap B) - P(A \cap B) - P(A \cap B) = \\[5pt]
                    &= P(A) + P(B) - P(A \cap B) \quad \text{\underline{q.e.d.}}
    \end{aligned}
\end{equation*}
