+ $M subset.eq Q$

  + (IA)
    - $0 in M$
    - $0 = 0^2 in Q$

  + (IS)

    Angenommen $x in M => x in Q$ ($x = n^2, n in NN$), folgt

    $
      x + 2sqrt(x) + 1 = n^2 + 2n + 1 = (n + 1)^2
    $

    Da $(n + 1)^2 in Q$ ist auch $x + 2sqrt(x) + 1 in Q$. Also gilt
    $M subset.eq Q$

+ $Q subset.eq M$

  + (IA)
    - $0 in M$
    - $0 = 0^2 in Q$

  + (IS)

    Angenommen $n^2 in Q => n^2 in M$, folgt

    $
      (n + 1)^2 = n^2 + 2n + 1 = n^2 + 2sqrt(n^2) + 1
    $

    Laut Bedingung $n^2 in M$ folgt, dass auch $n^2 + 2sqrt(n^2) + 1 in M$ gilt
    und somit auch $(n + 1)^2$

    Also gilt $Q subset.eq M$

$=>$ M = Q #h(1fr) #sym.square
